done for now (big_step norm)

stlc_norm/stlc.sig
@@ -1,8 +1,11 @@
 tm : Type
 ty : Type
 
-Lam : ty -> (bind tm in tm) -> tm
+T : tm
+F : tm
+If : tm -> tm -> tm -> tm
+Lam : ty -> (tm -> tm) -> tm
 App : tm -> tm -> tm
 
 Fun : ty -> ty -> ty
-Unit : ty
+Bool : ty
