stlc_norm/fintype.v
@@ -3,9 +3,7 @@
 
 Version: December 11, 2019.
 *)
-Require Import core.
-Require Import Setoid Morphisms Relation_Definitions.
-
+Require Export axioms.
 Set Implicit Arguments.
 Unset Strict Implicit.
 
@@ -30,9 +28,10 @@ Fixpoint fin (n : nat) : Type :=
 *)
 Definition ren (m n : nat) : Type := fin m -> fin n.
 
-Definition id {X} := @Datatypes.id X.
+Definition id {X} (x : X) := x.
 
-Definition idren {k: nat} : ren k k := @Datatypes.id (fin k).
+Definition idren {k: nat} : ren k k :=
+  fun x => x.
 
 (** We give a special name, to the newest element in a non-empty finite type, as it usually corresponds to a freshly bound variable. *)
 Definition var_zero {n : nat} : fin (S n) := None.
@@ -41,6 +40,8 @@ Definition null {T} (i : fin 0) : T := match i with end.
 
 Definition shift {n : nat} : ren n (S n) :=
   Some.
+
+Definition comp := @funcomp.
 
 (** Extension of Finite Mappings
     Assume we are given a mapping _f_ from _I^n_ to some type _X_, then we can _extend_ this mapping with a new value from _x : X_ to a mapping from _I^n+1_ to _X_. We denote this operation by _x . f_ and define it as follows:
@@ -51,8 +52,6 @@ Definition scons {X : Type} {n : nat} (x : X) (f : fin n -> X) (m : fin (S n)) :
   | Some i => f i
   end.
 
-#[ export ]
-Hint Opaque scons : rewrite.
 
 (** ** Type Class Instances for Notation *)
 
@@ -73,21 +72,23 @@ Class Ren4 (X1 X2 X3 X4 : Type) (Y Z : Type) :=
 Class Ren5 (X1 X2 X3 X4 X5 : Type) (Y Z : Type) :=
   ren5 : X1 -> X2 -> X3 -> X4 -> X5 -> Y -> Z.
 
-Module RenNotations.
-  Notation "s ⟨ xi1 ⟩" := (ren1  xi1 s) (at level 7, left associativity, format "s  ⟨ xi1 ⟩") : subst_scope.
+Declare Scope fscope. 
+Declare Scope subst_scope.
 
-  Notation "s ⟨ xi1 ; xi2 ⟩" := (ren2 xi1 xi2 s) (at level 7, left associativity, format "s  ⟨ xi1 ; xi2 ⟩") : subst_scope.
+Notation "s ⟨ xi1 ⟩" := (ren1  xi1 s) (at level 7, left associativity, format "s  ⟨ xi1 ⟩") : subst_scope.
 
-  Notation "s ⟨ xi1 ; xi2 ; xi3 ⟩" := (ren3 xi1 xi2 xi3 s) (at level 7, left associativity, format "s  ⟨ xi1 ; xi2 ; xi3 ⟩") : subst_scope.
+Notation "s ⟨ xi1 ; xi2 ⟩" := (ren2 xi1 xi2 s) (at level 7, left associativity, format "s  ⟨ xi1 ; xi2 ⟩") : subst_scope.
 
-  Notation "s ⟨ xi1 ; xi2 ; xi3 ; xi4 ⟩" := (ren4  xi1 xi2 xi3 xi4 s) (at level 7, left associativity, format "s  ⟨ xi1 ; xi2 ; xi3 ; xi4 ⟩") : subst_scope.
+Notation "s ⟨ xi1 ; xi2 ; xi3 ⟩" := (ren3 xi1 xi2 xi3 s) (at level 7, left associativity, format "s  ⟨ xi1 ; xi2 ; xi3 ⟩") : subst_scope.
 
-  Notation "s ⟨ xi1 ; xi2 ; xi3 ; xi4 ; xi5 ⟩" := (ren5  xi1 xi2 xi3 xi4 xi5 s) (at level 7, left associativity, format "s  ⟨ xi1 ; xi2 ; xi3 ; xi4 ; xi5 ⟩") : subst_scope.
+Notation "s ⟨ xi1 ; xi2 ; xi3 ; xi4 ⟩" := (ren4  xi1 xi2 xi3 xi4 s) (at level 7, left associativity, format "s  ⟨ xi1 ; xi2 ; xi3 ; xi4 ⟩") : subst_scope.
 
-  Notation "⟨ xi ⟩" := (ren1 xi) (at level 1, left associativity, format "⟨ xi ⟩") : fscope.
+Notation "s ⟨ xi1 ; xi2 ; xi3 ; xi4 ; xi5 ⟩" := (ren5  xi1 xi2 xi3 xi4 xi5 s) (at level 7, left associativity, format "s  ⟨ xi1 ; xi2 ; xi3 ; xi4 ; xi5 ⟩") : subst_scope.
 
-  Notation "⟨ xi1 ; xi2 ⟩" := (ren2 xi1 xi2) (at level 1, left associativity, format "⟨ xi1 ; xi2 ⟩") : fscope.
-End RenNotations.
+Notation "⟨ xi ⟩" := (ren1 xi) (at level 1, left associativity, format "⟨ xi ⟩") : fscope.
+
+Notation "⟨ xi1 ; xi2 ⟩" := (ren2 xi1 xi2) (at level 1, left associativity, format "⟨ xi1 ; xi2 ⟩") : fscope.
+
 
 (** *** Type Classes for Substiution *)
 
@@ -106,11 +107,9 @@ Class Subst4 (X1 X2 X3 X4: Type) (Y Z: Type) :=
 Class Subst5 (X1 X2 X3 X4 X5 : Type) (Y Z: Type) :=
   subst5 : X1 -> X2 -> X3 -> X4 -> X5  -> Y  -> Z.
 
-Module SubstNotations.
-  Notation "s [ sigma ]" := (subst1 sigma s) (at level 7, left associativity, format "s '/' [ sigma ]") : subst_scope.
+Notation "s [ sigma ]" := (subst1 sigma s) (at level 7, left associativity, format "s '/' [ sigma ]") : subst_scope.
 
-  Notation "s [ sigma ; tau ]" := (subst2 sigma tau s) (at level 7, left associativity, format "s '/' [ sigma ; '/'  tau ]") : subst_scope.
-End SubstNotations.
+Notation "s [ sigma ; tau ]" := (subst2 sigma tau s) (at level 7, left associativity, format "s '/' [ sigma ; '/'  tau ]") : subst_scope.
 
 (** ** Type Class for Variables *)
 Class Var X Y :=
@@ -123,24 +122,15 @@ Class Var X Y :=
     Substitutions represented as functions are ubiquitious in this development and we often have to compose them, without talking about their pointwise behaviour.
     That is, we are interested in the forward compostion of functions, _f o g_, for which we introduce a convenient notation, "f >> g". The direction of the arrow serves as a reminder of the _forward_ nature of this composition, that is first apply _f_, then _g_. *)
 
-Arguments funcomp {X Y Z} (g)%_fscope (f)%_fscope.
+Arguments funcomp {X Y Z} (g)%fscope (f)%fscope.
 
-Module CombineNotations.
-  Notation "f >> g" := (funcomp g f) (at level 50) : fscope.
+Notation "f >> g" := (funcomp g f) (at level 50).
+Open Scope subst_scope.
 
-  Notation "s .: sigma" := (scons s sigma) (at level 55, sigma at next level, right associativity) : subst_scope.
-
-  #[ global ]
-  Open Scope fscope.
-  #[ global ]
-  Open Scope subst_scope.
-End CombineNotations.
-
-Import CombineNotations.
-
+Notation "x .: f" := (@scons _ _ x f) (at level 55) : subst_scope.
 
 (** Generic lifting operation for renamings *)
-Definition up_ren {m n} (xi : ren m n) : ren (S m) (S n) :=
+Definition up_ren m n (xi : ren m n) : ren (S m) (S n) :=
   var_zero .: xi >> shift.
 
 (** Generic proof that lifting of renamings composes. *)
@@ -148,59 +138,30 @@ Lemma up_ren_ren k l m (xi: ren k l) (zeta : ren l m) (rho: ren k m) (E: forall 
   forall x, (up_ren xi >> up_ren zeta) x = up_ren rho x.
 Proof.
   intros [x|].
-  - cbn. unfold funcomp. now rewrite <- E.
+  - simpl. unfold funcomp. now rewrite <- E.
   - reflexivity.
 Qed.
 
 Arguments up_ren_ren {k l m} xi zeta rho E.
 
+Lemma scons_eta {T} {n : nat} (f : fin (S n) -> T) :
+  f var_zero .: shift >> f = f.
+Proof. fext. intros [x|]; reflexivity.  Qed.
+
+
+Lemma scons_eta_id {n : nat} : var_zero .: shift = id :> (fin (S n) -> fin (S n)).
+Proof. fext. intros [x|]; reflexivity. Qed.
+
+Lemma scons_comp (T: Type) U {m} (s: T) (sigma: fin m -> T) (tau: T -> U ) :
+  (s .: sigma) >> tau = (tau s) .: (sigma >> tau) .
+Proof.
+  fext. intros [x|]. reflexivity. simpl. reflexivity.
+Qed.
+
 Lemma fin_eta {X} (f g : fin 0 -> X) :
-  pointwise_relation _ eq f g.
+  forall x, f x = g x.
 Proof. intros []. Qed.
 
-(** Eta laws *)
-Lemma scons_eta' {T} {n : nat} (f : fin (S n) -> T) :
-  pointwise_relation _ eq (f var_zero .: (funcomp f shift)) f.
-Proof. intros x. destruct x; reflexivity. Qed.
-
-Lemma scons_eta_id' {n : nat} :
-  pointwise_relation (fin (S n)) eq (var_zero .: shift) id.
-Proof. intros x. destruct x; reflexivity. Qed.
-
-Lemma scons_comp' {T:Type} {U} {m} (s: T) (sigma: fin m -> T) (tau: T -> U) :
-  pointwise_relation _ eq (funcomp tau (s .: sigma)) ((tau s) .: (funcomp tau sigma)).
-Proof. intros x. destruct x; reflexivity. Qed.
-
-(* Lemma scons_tail'_pointwise {X} {n} (s : X) (f : fin n -> X) : *)
-(*   pointwise_relation _ eq (funcomp (scons s f) shift) f. *)
-(* Proof. *)
-(*   reflexivity. *)
-(* Qed. *)
-
-(* Lemma scons_tail' {X} {n} (s : X) (f : fin n -> X) x : *)
-(*   (scons s f (shift x)) = f x. *)
-(* Proof. *)
-(*   reflexivity. *)
-(* Qed. *)
-
-(* Morphism for Setoid Rewriting. The only morphism that can be defined statically. *)
-#[export] Instance scons_morphism {X: Type} {n:nat} :
-  Proper (eq ==> pointwise_relation _ eq ==> pointwise_relation _ eq) (@scons X n).
-Proof.
-  intros t t' -> sigma tau H.
-  intros [x|].
-  cbn. apply H.
-  reflexivity.
-Qed.
-
-#[export] Instance scons_morphism2 {X: Type} {n: nat} :
-  Proper (eq ==> pointwise_relation _ eq ==> eq ==> eq) (@scons X n).
-Proof.
-  intros ? t -> sigma tau H ? x ->.
-  destruct x as [x|].
-  cbn. apply H.
-  reflexivity.
-Qed.
 
 (** ** Variadic Substitution Primitives *)
 
@@ -221,35 +182,6 @@ Proof.
       * exact g.
 Defined.
 
-#[export] Hint Opaque scons_p : rewrite.
-
-#[export] Instance scons_p_morphism {X: Type} {m n:nat} :
-  Proper (pointwise_relation _ eq ==> pointwise_relation _ eq ==> pointwise_relation _ eq) (@scons_p X m n).
-Proof.
-  intros sigma sigma' Hsigma tau tau' Htau.
-  intros x.
-  induction m.
-  - cbn. apply Htau.
-  - cbn. change (fin (S m + n)) with (fin (S (m + n))) in x.
-    destruct x as [x|].
-    + cbn. apply IHm.
-      intros ?. apply Hsigma.
-    + cbn. apply Hsigma.
-Qed.
-
-#[export] Instance scons_p_morphism2 {X: Type} {m n:nat} :
-  Proper (pointwise_relation _ eq ==> pointwise_relation _ eq ==> eq ==> eq) (@scons_p X m n).
-Proof.
-  intros sigma sigma' Hsigma tau tau' Htau ? x ->.
-  induction m.
-  - cbn. apply Htau.
-  - cbn. change (fin (S m + n)) with (fin (S (m + n))) in x.
-    destruct x as [x|].
-    + cbn. apply IHm.
-      intros ?. apply Hsigma.
-    + cbn. apply Hsigma.
-Qed.
-
 Definition zero_p {m : nat} {n} : fin m -> fin (m + n).
 Proof.
   induction m.
@@ -269,25 +201,17 @@ Proof.
     + reflexivity.
 Qed.
 
-Lemma scons_p_head_pointwise {X} {m n} (f : fin m -> X) (g : fin n -> X) :
-  pointwise_relation _ eq (funcomp (scons_p f g) zero_p) f.
-Proof.
-  intros z.
-  unfold funcomp.
-  induction m.
-  - inversion z.
-  - destruct z.
-    + simpl. now rewrite IHm.
-    + reflexivity.
-Qed.
+Lemma scons_p_head X m n (f : fin m -> X) (g : fin n -> X) :
+  (zero_p  >> scons_p f g) = f.
+Proof. fext. intros z. unfold funcomp. apply scons_p_head'. Qed.
 
 Lemma scons_p_tail' X  m n (f : fin m -> X) (g : fin n -> X) z :
   scons_p  f g (shift_p m z) = g z.
 Proof. induction m; cbn; eauto. Qed.
 
-Lemma scons_p_tail_pointwise X  m n (f : fin m -> X) (g : fin n -> X) :
-  pointwise_relation _ eq (funcomp (scons_p f g) (shift_p m)) g.
-Proof. intros z. induction m; cbn; eauto. Qed.
+Lemma scons_p_tail X  m n (f : fin m -> X) (g : fin n -> X) :
+  shift_p m  >> scons_p f g = g.
+Proof. fext. intros z. unfold funcomp. apply scons_p_tail'. Qed.
 
 Lemma destruct_fin {m n} (x : fin (m + n)):
   (exists x', x = zero_p  x') \/ exists x', x = shift_p m x'.
@@ -301,23 +225,17 @@ Proof.
     + left. exists None. eauto.
 Qed.
 
-Lemma scons_p_comp' X Y m n (f : fin m -> X) (g : fin n -> X) (h : X -> Y) :
-  pointwise_relation _ eq (funcomp h (scons_p f g)) (scons_p (f >> h) (g >> h)).
+Lemma scons_p_comp' X Y m n (f : fin m -> X) (g : fin n -> X) (h : X -> Y) x:
+ h (scons_p  f g x)  = scons_p (f >> h) (g >> h) x.
 Proof.
-  intros x.
   destruct (destruct_fin x) as [[x' ->]|[x' ->]].
-  (* TODO better way to solve this? *)
-  - revert x'.
-    apply pointwise_forall.
-    change (fun x => (scons_p f g >> h) (zero_p x)) with (zero_p >> scons_p f g >> h).
-    now setoid_rewrite scons_p_head_pointwise.
-  - revert x'.
-    apply pointwise_forall.
-    change (fun x => (scons_p f g >> h) (shift_p m x)) with (shift_p m >> scons_p f g >> h).
-    change (fun x => scons_p (f >> h) (g >> h) (shift_p m x)) with (shift_p m >> scons_p (f >> h) (g >> h)).
-    now rewrite !scons_p_tail_pointwise.
+  - now rewrite !scons_p_head'.
+  - now rewrite !scons_p_tail'.
 Qed.
 
+Lemma scons_p_comp {X Y m n} {f : fin m -> X} {g : fin n -> X} {h : X -> Y} :
+  (scons_p f g) >> h = scons_p   (f >> h) (g >> h).
+Proof. fext. intros z. unfold funcomp. apply scons_p_comp'. Qed.
 
 Lemma scons_p_congr {X} {m n} (f f' : fin m -> X) (g g': fin n -> X) z:
   (forall x, f x = f' x) -> (forall x, g x = g' x) -> scons_p f g z = scons_p f' g' z.
@@ -355,27 +273,90 @@ Qed.
 Arguments scons_p_eta {X} {m n} {f g} h {z}.
 Arguments scons_p_congr {X} {m n} {f f'} {g g'} {z}.
 
+Opaque scons.
+Opaque var_zero.
+Opaque null.
+Opaque shift.
+Opaque up_ren.
+Opaque var_zero.
+Opaque idren.
+Opaque comp.
+Opaque funcomp.
+Opaque id.
+
+
 (** ** Notations for Scoped Syntax *)
 
-Module ScopedNotations.
-  Include RenNotations.
-  Include SubstNotations.
-  Include CombineNotations.
+Module CommaNotation.
+Notation "s , sigma" := (scons s sigma) (at level 60, format "s ,  sigma", right associativity) : subst_scope.
+End CommaNotation.
 
-(* Notation "s , sigma" := (scons s sigma) (at level 60, format "s ,  sigma", right associativity) : subst_scope. *)
+Notation "s '..'" := (scons s ids) (at level 1, format "s ..") : subst_scope.
 
-  Notation "s '..'" := (scons s ids) (at level 1, format "s ..") : subst_scope.
+Notation "↑" := (shift) : subst_scope.
 
-  Notation "↑" := (shift) : subst_scope.
-
-  #[global]
-  Open Scope fscope.
-  #[global]
-  Open Scope subst_scope.
-End ScopedNotations.
+Ltac unfold_funcomp := match goal with
+                           | |-  context[(?f >> ?g) ?s] => change ((f >> g) s) with (g (f s))
+                           end.
 
 
 (** ** Tactics for Scoped Syntax *)
+
+(** Generic fsimpl tactic: simplifies the above primitives in a goal. *)
+Ltac fsimpl :=
+  repeat match goal with
+         | [|- context[id >> ?f]] => change (id >> f) with f (* AsimplCompIdL *)
+         | [|- context[?f >> id]] => change (f >> id) with f (* AsimplCompIdR *)
+         | [|- context [id ?s]] => change (id s) with s
+         | [|- context[comp ?f ?g]] => change (comp f g) with (g >> f) (* AsimplCompIdL *)
+         | [|- context[(?f >> ?g) >> ?h]] =>
+           change ((f >> g) >> h) with (f >> (g >> h)) (* AsimplComp *)
+
+         | [|- zero_p >> scons_p ?f ?g] => rewrite scons_p_head
+
+         | [|- context[(?s.:?sigma) var_zero]] => change ((s.:sigma) var_zero) with s
+         | [|- context[(?s.:?sigma) (shift ?m)]] => change ((s.:sigma) (shift m)) with (sigma m)
+
+         | [|- context[idren >> ?f]] => change (idren >> f) with f
+         | [|- context[?f >> idren]] => change (f >> idren) with f
+         | [|- context[?f >> (?x .: ?g)]] => change (f >> (x .: g)) with g
+         | [|- context[?x2 .: shift >> ?f]] => change x2 with (f var_zero); rewrite (@scons_eta _ _ f)
+         | [|- context[?f var_zero .: ?g]] => change g with (shift >> f); rewrite scons_eta
+
+         |[|- _ =  ?h (?f ?s)] => change (h (f s)) with ((f >> h) s)
+         |[|-  ?h (?f ?s) = _] => change (h (f s)) with ((f >> h) s)
+
+         | _ => first [progress (rewrite scons_comp) |  progress (rewrite scons_eta_id) | progress (autorewrite with FunctorInstances)]
+         end.
+
+(** Generic fsimpl tactic: simplifies the above primitives in the context *)
+Ltac fsimplc :=
+  repeat match goal with
+         | [H: context[id >> ?f] |- _] => change (id >> f) with f in H(* AsimplCompIdL *)
+         | [H: context[?f >> id]|- _] => change (f >> id) with f in H(* AsimplCompIdR *)
+         | [H: context [id ?s]|- _] => change (id s) with s in H
+         | [H: context[comp ?f ?g]|- _] => change (comp f g) with (g >> f) in H (* AsimplCompIdL *)
+         | [H: context[(?f >> ?g) >> ?h]|- _] =>
+           change ((f >> g) >> h) with (f >> (g >> h)) in H (* AsimplComp *)
+         | [H: context[(?s.:?sigma) var_zero]|- _] => change ((s.:sigma) var_zero) with s in H
+         | [H: context[(?s.:?sigma) var_zero]|- _] => change ((s.:sigma) var_zero) with s in H
+         | [H: context[(?s.:?sigma) (shift ?m)]|- _] => change ((s.:sigma) (shift m)) with (sigma m) in H
+                                                                                      |[H : context[ _ =  ?h (?f ?s)]|- _] => change (h (f s)) with ((f >> h) s) in H
+         |[H: context[?h (?f ?s) = _]|- _] => change (h (f s)) with ((f >> h) s) in H
+         | [H: context[idren >> ?f]|- _] => change (idren >> f) with f in H
+         | [H: context[?f >> idren]|- _] => change (f >> idren) with f in H
+         | [H: context[?f >> (?x .: ?g)]|- _] =>
+           change (f >> (x .: g)) with g in H
+         | [H: context[?x2 .: shift >> ?f]|- _] =>
+           change x2 with (f var_zero) in H; rewrite (@scons_eta _ _ f) in H
+         | [H: context[?f var_zero .: ?g]|- _] =>
+           change g with (shift >> f) in H; rewrite scons_eta in H
+         | _ => first [progress (rewrite scons_comp in *) | progress (rewrite scons_eta_id in *) | progress (autorewrite with FunctorInstances in *)]
+         end.
+
+(** Simplification in both the goal and the context *)
+Tactic Notation "fsimpl" "in" "*" :=
+  fsimpl; fsimplc.
 
 Tactic Notation "auto_case" tactic(t) :=  (match goal with
                                            | [|- forall (i : fin 0), _] => intros []; t
@@ -385,35 +366,6 @@ Tactic Notation "auto_case" tactic(t) :=  (match goal with
                                            | [|- forall (i : fin (S _)), _] =>  intros [?|]; t
                                            end).
 
-#[export] Hint Rewrite @scons_p_head' @scons_p_tail' : FunctorInstances.
 
-(** Generic fsimpl tactic: simplifies the above primitives in a goal. *)
-Ltac fsimpl :=
-  repeat match goal with
-         | [|- context[id >> ?f]] => change (id >> f) with f (* AsimplCompIdL *)
-         | [|- context[?f >> id]] => change (f >> id) with f (* AsimplCompIdR *)
-         | [|- context [id ?s]] => change (id s) with s
-         | [|- context[(?f >> ?g) >> ?h]] => change ((f >> g) >> h) with (f >> (g >> h)) (* AsimplComp *)
-         (* | [|- zero_p >> scons_p ?f ?g] => rewrite scons_p_head *)
-         | [|- context[(?s .: ?sigma) var_zero]] => change ((s.:sigma) var_zero) with s
-         | [|- context[(?s .: ?sigma) (shift ?m)]] => change ((s.:sigma) (shift m)) with (sigma m)
-           (* first [progress setoid_rewrite scons_tail' | progress setoid_rewrite scons_tail'_pointwise ] *)
-         | [|- context[idren >> ?f]] => change (idren >> f) with f
-         | [|- context[?f >> idren]] => change (f >> idren) with f
-         | [|- context[?f >> (?x .: ?g)]] => change (f >> (x .: g)) with g (* f should evaluate to shift *)
-         | [|- context[?x2 .: (funcomp ?f shift)]] => change (scons x2 (funcomp f shift)) with (scons (f var_zero) (funcomp f shift)); setoid_rewrite (@scons_eta' _ _ f); eta_reduce
-         | [|- context[?f var_zero .: ?g]] => change (scons (f var_zero) g) with (scons (f var_zero) (funcomp f shift)); setoid_rewrite scons_eta'; eta_reduce
-         | [|- _ =  ?h (?f ?s)] => change (h (f s)) with ((f >> h) s)
-         | [|-  ?h (?f ?s) = _] => change (h (f s)) with ((f >> h) s)
-         | [|- context[funcomp _ (scons _ _)]] => setoid_rewrite scons_comp'; eta_reduce
-         | [|- context[funcomp _ (scons_p _ _ _)]] => setoid_rewrite scons_p_comp'; eta_reduce
-         | [|- context[scons (@var_zero _) shift]] => setoid_rewrite scons_eta_id'; eta_reduce
-         (* | _ => progress autorewrite with FunctorInstances *)
-         | [|- context[funcomp (scons_p _ _ _) (zero_p _)]] =>
-           first [progress setoid_rewrite scons_p_head_pointwise | progress setoid_rewrite scons_p_head' ]
-         | [|- context[scons_p _ _ _ (zero_p _ _)]] => setoid_rewrite scons_p_head'
-         | [|- context[funcomp (scons_p _ _ _) (shift_p _)]] =>
-           first [progress setoid_rewrite scons_p_tail_pointwise | progress setoid_rewrite scons_p_tail' ]
-         | [|- context[scons_p _ _ _ (shift_p _ _)]] => setoid_rewrite scons_p_tail'
-         | _ => first [progress minimize | progress cbn [shift scons scons_p] ]
-         end.
+(** Functor instances which can be added later on. *)
+Hint Rewrite  @scons_p_comp scons_p_head scons_p_tail @scons_p_head' @scons_p_tail': FunctorInstances.
