stlc_norm/stlc.v
@@ -1,713 +1,290 @@
-Require Import core fintype.
-
-Require Import Setoid Morphisms Relation_Definitions.
+Require Export fintype.
 
 
-Module Core.
 
-Inductive ty : Type :=
-  | Fun : ty -> ty -> ty
-  | Unit : ty.
+Section ty.
+Inductive ty  : Type :=
+  | Fun : ty   -> ty   -> ty 
+  | Bool : ty .
 
-Lemma congr_Fun {s0 : ty} {s1 : ty} {t0 : ty} {t1 : ty} (H0 : s0 = t0)
-  (H1 : s1 = t1) : Fun s0 s1 = Fun t0 t1.
-Proof.
-exact (eq_trans (eq_trans eq_refl (ap (fun x => Fun x s1) H0))
-         (ap (fun x => Fun t0 x) H1)).
-Qed.
+Lemma congr_Fun  { s0 : ty   } { s1 : ty   } { t0 : ty   } { t1 : ty   } (H1 : s0 = t0) (H2 : s1 = t1) : Fun s0 s1 = Fun t0 t1 .
+Proof. congruence. Qed.
 
-Lemma congr_Unit : Unit = Unit.
-Proof.
-exact (eq_refl).
-Qed.
+Lemma congr_Bool  : Bool  = Bool  .
+Proof. congruence. Qed.
 
-Inductive tm (n_tm : nat) : Type :=
-  | var_tm : fin n_tm -> tm n_tm
-  | Lam : ty -> tm (S n_tm) -> tm n_tm
-  | App : tm n_tm -> tm n_tm -> tm n_tm.
+End ty.
 
-Lemma congr_Lam {m_tm : nat} {s0 : ty} {s1 : tm (S m_tm)} {t0 : ty}
-  {t1 : tm (S m_tm)} (H0 : s0 = t0) (H1 : s1 = t1) :
-  Lam m_tm s0 s1 = Lam m_tm t0 t1.
-Proof.
-exact (eq_trans (eq_trans eq_refl (ap (fun x => Lam m_tm x s1) H0))
-         (ap (fun x => Lam m_tm t0 x) H1)).
-Qed.
+Section tm.
+Inductive tm (ntm : nat) : Type :=
+  | var_tm : (fin) (ntm) -> tm (ntm)
+  | T : tm (ntm)
+  | F : tm (ntm)
+  | If : tm  (ntm) -> tm  (ntm) -> tm  (ntm) -> tm (ntm)
+  | Lam : ty   -> tm  ((S) ntm) -> tm (ntm)
+  | App : tm  (ntm) -> tm  (ntm) -> tm (ntm).
 
-Lemma congr_App {m_tm : nat} {s0 : tm m_tm} {s1 : tm m_tm} {t0 : tm m_tm}
-  {t1 : tm m_tm} (H0 : s0 = t0) (H1 : s1 = t1) :
-  App m_tm s0 s1 = App m_tm t0 t1.
-Proof.
-exact (eq_trans (eq_trans eq_refl (ap (fun x => App m_tm x s1) H0))
-         (ap (fun x => App m_tm t0 x) H1)).
-Qed.
+Lemma congr_T { mtm : nat } : T (mtm) = T (mtm) .
+Proof. congruence. Qed.
 
-Lemma upRen_tm_tm {m : nat} {n : nat} (xi : fin m -> fin n) :
-  fin (S m) -> fin (S n).
-Proof.
-exact (up_ren xi).
-Defined.
+Lemma congr_F { mtm : nat } : F (mtm) = F (mtm) .
+Proof. congruence. Qed.
 
-Lemma upRen_list_tm_tm (p : nat) {m : nat} {n : nat} (xi : fin m -> fin n) :
-  fin (plus p m) -> fin (plus p n).
-Proof.
-exact (upRen_p p xi).
-Defined.
+Lemma congr_If { mtm : nat } { s0 : tm  (mtm) } { s1 : tm  (mtm) } { s2 : tm  (mtm) } { t0 : tm  (mtm) } { t1 : tm  (mtm) } { t2 : tm  (mtm) } (H1 : s0 = t0) (H2 : s1 = t1) (H3 : s2 = t2) : If (mtm) s0 s1 s2 = If (mtm) t0 t1 t2 .
+Proof. congruence. Qed.
 
-Fixpoint ren_tm {m_tm : nat} {n_tm : nat} (xi_tm : fin m_tm -> fin n_tm)
-(s : tm m_tm) {struct s} : tm n_tm :=
-  match s with
-  | var_tm _ s0 => var_tm n_tm (xi_tm s0)
-  | Lam _ s0 s1 => Lam n_tm s0 (ren_tm (upRen_tm_tm xi_tm) s1)
-  | App _ s0 s1 => App n_tm (ren_tm xi_tm s0) (ren_tm xi_tm s1)
+Lemma congr_Lam { mtm : nat } { s0 : ty   } { s1 : tm  ((S) mtm) } { t0 : ty   } { t1 : tm  ((S) mtm) } (H1 : s0 = t0) (H2 : s1 = t1) : Lam (mtm) s0 s1 = Lam (mtm) t0 t1 .
+Proof. congruence. Qed.
+
+Lemma congr_App { mtm : nat } { s0 : tm  (mtm) } { s1 : tm  (mtm) } { t0 : tm  (mtm) } { t1 : tm  (mtm) } (H1 : s0 = t0) (H2 : s1 = t1) : App (mtm) s0 s1 = App (mtm) t0 t1 .
+Proof. congruence. Qed.
+
+Definition upRen_tm_tm { m : nat } { n : nat } (xi : (fin) (m) -> (fin) (n)) : (fin) ((S) (m)) -> (fin) ((S) (n)) :=
+  (up_ren) xi.
+
+Fixpoint ren_tm { mtm : nat } { ntm : nat } (xitm : (fin) (mtm) -> (fin) (ntm)) (s : tm (mtm)) : tm (ntm) :=
+    match s return tm (ntm) with
+    | var_tm (_) s => (var_tm (ntm)) (xitm s)
+    | T (_)  => T (ntm)
+    | F (_)  => F (ntm)
+    | If (_) s0 s1 s2 => If (ntm) ((ren_tm xitm) s0) ((ren_tm xitm) s1) ((ren_tm xitm) s2)
+    | Lam (_) s0 s1 => Lam (ntm) ((fun x => x) s0) ((ren_tm (upRen_tm_tm xitm)) s1)
+    | App (_) s0 s1 => App (ntm) ((ren_tm xitm) s0) ((ren_tm xitm) s1)
+    end.
+
+Definition up_tm_tm { m : nat } { ntm : nat } (sigma : (fin) (m) -> tm (ntm)) : (fin) ((S) (m)) -> tm ((S) ntm) :=
+  (scons) ((var_tm ((S) ntm)) (var_zero)) ((funcomp) (ren_tm (shift)) sigma).
+
+Fixpoint subst_tm { mtm : nat } { ntm : nat } (sigmatm : (fin) (mtm) -> tm (ntm)) (s : tm (mtm)) : tm (ntm) :=
+    match s return tm (ntm) with
+    | var_tm (_) s => sigmatm s
+    | T (_)  => T (ntm)
+    | F (_)  => F (ntm)
+    | If (_) s0 s1 s2 => If (ntm) ((subst_tm sigmatm) s0) ((subst_tm sigmatm) s1) ((subst_tm sigmatm) s2)
+    | Lam (_) s0 s1 => Lam (ntm) ((fun x => x) s0) ((subst_tm (up_tm_tm sigmatm)) s1)
+    | App (_) s0 s1 => App (ntm) ((subst_tm sigmatm) s0) ((subst_tm sigmatm) s1)
+    end.
+
+Definition upId_tm_tm { mtm : nat } (sigma : (fin) (mtm) -> tm (mtm)) (Eq : forall x, sigma x = (var_tm (mtm)) x) : forall x, (up_tm_tm sigma) x = (var_tm ((S) mtm)) x :=
+  fun n => match n with
+  | Some fin_n => (ap) (ren_tm (shift)) (Eq fin_n)
+  | None  => eq_refl
   end.
 
-Lemma up_tm_tm {m : nat} {n_tm : nat} (sigma : fin m -> tm n_tm) :
-  fin (S m) -> tm (S n_tm).
-Proof.
-exact (scons (var_tm (S n_tm) var_zero) (funcomp (ren_tm shift) sigma)).
-Defined.
+Fixpoint idSubst_tm { mtm : nat } (sigmatm : (fin) (mtm) -> tm (mtm)) (Eqtm : forall x, sigmatm x = (var_tm (mtm)) x) (s : tm (mtm)) : subst_tm sigmatm s = s :=
+    match s return subst_tm sigmatm s = s with
+    | var_tm (_) s => Eqtm s
+    | T (_)  => congr_T 
+    | F (_)  => congr_F 
+    | If (_) s0 s1 s2 => congr_If ((idSubst_tm sigmatm Eqtm) s0) ((idSubst_tm sigmatm Eqtm) s1) ((idSubst_tm sigmatm Eqtm) s2)
+    | Lam (_) s0 s1 => congr_Lam ((fun x => (eq_refl) x) s0) ((idSubst_tm (up_tm_tm sigmatm) (upId_tm_tm (_) Eqtm)) s1)
+    | App (_) s0 s1 => congr_App ((idSubst_tm sigmatm Eqtm) s0) ((idSubst_tm sigmatm Eqtm) s1)
+    end.
 
-Lemma up_list_tm_tm (p : nat) {m : nat} {n_tm : nat}
-  (sigma : fin m -> tm n_tm) : fin (plus p m) -> tm (plus p n_tm).
-Proof.
-exact (scons_p p (funcomp (var_tm (plus p n_tm)) (zero_p p))
-         (funcomp (ren_tm (shift_p p)) sigma)).
-Defined.
-
-Fixpoint subst_tm {m_tm : nat} {n_tm : nat} (sigma_tm : fin m_tm -> tm n_tm)
-(s : tm m_tm) {struct s} : tm n_tm :=
-  match s with
-  | var_tm _ s0 => sigma_tm s0
-  | Lam _ s0 s1 => Lam n_tm s0 (subst_tm (up_tm_tm sigma_tm) s1)
-  | App _ s0 s1 => App n_tm (subst_tm sigma_tm s0) (subst_tm sigma_tm s1)
+Definition upExtRen_tm_tm { m : nat } { n : nat } (xi : (fin) (m) -> (fin) (n)) (zeta : (fin) (m) -> (fin) (n)) (Eq : forall x, xi x = zeta x) : forall x, (upRen_tm_tm xi) x = (upRen_tm_tm zeta) x :=
+  fun n => match n with
+  | Some fin_n => (ap) (shift) (Eq fin_n)
+  | None  => eq_refl
   end.
 
-Lemma upId_tm_tm {m_tm : nat} (sigma : fin m_tm -> tm m_tm)
-  (Eq : forall x, sigma x = var_tm m_tm x) :
-  forall x, up_tm_tm sigma x = var_tm (S m_tm) x.
-Proof.
-exact (fun n =>
-       match n with
-       | Some fin_n => ap (ren_tm shift) (Eq fin_n)
-       | None => eq_refl
-       end).
-Qed.
+Fixpoint extRen_tm { mtm : nat } { ntm : nat } (xitm : (fin) (mtm) -> (fin) (ntm)) (zetatm : (fin) (mtm) -> (fin) (ntm)) (Eqtm : forall x, xitm x = zetatm x) (s : tm (mtm)) : ren_tm xitm s = ren_tm zetatm s :=
+    match s return ren_tm xitm s = ren_tm zetatm s with
+    | var_tm (_) s => (ap) (var_tm (ntm)) (Eqtm s)
+    | T (_)  => congr_T 
+    | F (_)  => congr_F 
+    | If (_) s0 s1 s2 => congr_If ((extRen_tm xitm zetatm Eqtm) s0) ((extRen_tm xitm zetatm Eqtm) s1) ((extRen_tm xitm zetatm Eqtm) s2)
+    | Lam (_) s0 s1 => congr_Lam ((fun x => (eq_refl) x) s0) ((extRen_tm (upRen_tm_tm xitm) (upRen_tm_tm zetatm) (upExtRen_tm_tm (_) (_) Eqtm)) s1)
+    | App (_) s0 s1 => congr_App ((extRen_tm xitm zetatm Eqtm) s0) ((extRen_tm xitm zetatm Eqtm) s1)
+    end.
 
-Lemma upId_list_tm_tm {p : nat} {m_tm : nat} (sigma : fin m_tm -> tm m_tm)
-  (Eq : forall x, sigma x = var_tm m_tm x) :
-  forall x, up_list_tm_tm p sigma x = var_tm (plus p m_tm) x.
-Proof.
-exact (fun n =>
-       scons_p_eta (var_tm (plus p m_tm))
-         (fun n => ap (ren_tm (shift_p p)) (Eq n)) (fun n => eq_refl)).
-Qed.
-
-Fixpoint idSubst_tm {m_tm : nat} (sigma_tm : fin m_tm -> tm m_tm)
-(Eq_tm : forall x, sigma_tm x = var_tm m_tm x) (s : tm m_tm) {struct s} :
-subst_tm sigma_tm s = s :=
-  match s with
-  | var_tm _ s0 => Eq_tm s0
-  | Lam _ s0 s1 =>
-      congr_Lam (eq_refl s0)
-        (idSubst_tm (up_tm_tm sigma_tm) (upId_tm_tm _ Eq_tm) s1)
-  | App _ s0 s1 =>
-      congr_App (idSubst_tm sigma_tm Eq_tm s0) (idSubst_tm sigma_tm Eq_tm s1)
+Definition upExt_tm_tm { m : nat } { ntm : nat } (sigma : (fin) (m) -> tm (ntm)) (tau : (fin) (m) -> tm (ntm)) (Eq : forall x, sigma x = tau x) : forall x, (up_tm_tm sigma) x = (up_tm_tm tau) x :=
+  fun n => match n with
+  | Some fin_n => (ap) (ren_tm (shift)) (Eq fin_n)
+  | None  => eq_refl
   end.
 
-Lemma upExtRen_tm_tm {m : nat} {n : nat} (xi : fin m -> fin n)
-  (zeta : fin m -> fin n) (Eq : forall x, xi x = zeta x) :
-  forall x, upRen_tm_tm xi x = upRen_tm_tm zeta x.
-Proof.
-exact (fun n =>
-       match n with
-       | Some fin_n => ap shift (Eq fin_n)
-       | None => eq_refl
-       end).
-Qed.
+Fixpoint ext_tm { mtm : nat } { ntm : nat } (sigmatm : (fin) (mtm) -> tm (ntm)) (tautm : (fin) (mtm) -> tm (ntm)) (Eqtm : forall x, sigmatm x = tautm x) (s : tm (mtm)) : subst_tm sigmatm s = subst_tm tautm s :=
+    match s return subst_tm sigmatm s = subst_tm tautm s with
+    | var_tm (_) s => Eqtm s
+    | T (_)  => congr_T 
+    | F (_)  => congr_F 
+    | If (_) s0 s1 s2 => congr_If ((ext_tm sigmatm tautm Eqtm) s0) ((ext_tm sigmatm tautm Eqtm) s1) ((ext_tm sigmatm tautm Eqtm) s2)
+    | Lam (_) s0 s1 => congr_Lam ((fun x => (eq_refl) x) s0) ((ext_tm (up_tm_tm sigmatm) (up_tm_tm tautm) (upExt_tm_tm (_) (_) Eqtm)) s1)
+    | App (_) s0 s1 => congr_App ((ext_tm sigmatm tautm Eqtm) s0) ((ext_tm sigmatm tautm Eqtm) s1)
+    end.
 
-Lemma upExtRen_list_tm_tm {p : nat} {m : nat} {n : nat} (xi : fin m -> fin n)
-  (zeta : fin m -> fin n) (Eq : forall x, xi x = zeta x) :
-  forall x, upRen_list_tm_tm p xi x = upRen_list_tm_tm p zeta x.
-Proof.
-exact (fun n =>
-       scons_p_congr (fun n => eq_refl) (fun n => ap (shift_p p) (Eq n))).
-Qed.
+Definition up_ren_ren_tm_tm { k : nat } { l : nat } { m : nat } (xi : (fin) (k) -> (fin) (l)) (tau : (fin) (l) -> (fin) (m)) (theta : (fin) (k) -> (fin) (m)) (Eq : forall x, ((funcomp) tau xi) x = theta x) : forall x, ((funcomp) (upRen_tm_tm tau) (upRen_tm_tm xi)) x = (upRen_tm_tm theta) x :=
+  up_ren_ren xi tau theta Eq.
 
-Fixpoint extRen_tm {m_tm : nat} {n_tm : nat} (xi_tm : fin m_tm -> fin n_tm)
-(zeta_tm : fin m_tm -> fin n_tm) (Eq_tm : forall x, xi_tm x = zeta_tm x)
-(s : tm m_tm) {struct s} : ren_tm xi_tm s = ren_tm zeta_tm s :=
-  match s with
-  | var_tm _ s0 => ap (var_tm n_tm) (Eq_tm s0)
-  | Lam _ s0 s1 =>
-      congr_Lam (eq_refl s0)
-        (extRen_tm (upRen_tm_tm xi_tm) (upRen_tm_tm zeta_tm)
-           (upExtRen_tm_tm _ _ Eq_tm) s1)
-  | App _ s0 s1 =>
-      congr_App (extRen_tm xi_tm zeta_tm Eq_tm s0)
-        (extRen_tm xi_tm zeta_tm Eq_tm s1)
+Fixpoint compRenRen_tm { ktm : nat } { ltm : nat } { mtm : nat } (xitm : (fin) (mtm) -> (fin) (ktm)) (zetatm : (fin) (ktm) -> (fin) (ltm)) (rhotm : (fin) (mtm) -> (fin) (ltm)) (Eqtm : forall x, ((funcomp) zetatm xitm) x = rhotm x) (s : tm (mtm)) : ren_tm zetatm (ren_tm xitm s) = ren_tm rhotm s :=
+    match s return ren_tm zetatm (ren_tm xitm s) = ren_tm rhotm s with
+    | var_tm (_) s => (ap) (var_tm (ltm)) (Eqtm s)
+    | T (_)  => congr_T 
+    | F (_)  => congr_F 
+    | If (_) s0 s1 s2 => congr_If ((compRenRen_tm xitm zetatm rhotm Eqtm) s0) ((compRenRen_tm xitm zetatm rhotm Eqtm) s1) ((compRenRen_tm xitm zetatm rhotm Eqtm) s2)
+    | Lam (_) s0 s1 => congr_Lam ((fun x => (eq_refl) x) s0) ((compRenRen_tm (upRen_tm_tm xitm) (upRen_tm_tm zetatm) (upRen_tm_tm rhotm) (up_ren_ren (_) (_) (_) Eqtm)) s1)
+    | App (_) s0 s1 => congr_App ((compRenRen_tm xitm zetatm rhotm Eqtm) s0) ((compRenRen_tm xitm zetatm rhotm Eqtm) s1)
+    end.
+
+Definition up_ren_subst_tm_tm { k : nat } { l : nat } { mtm : nat } (xi : (fin) (k) -> (fin) (l)) (tau : (fin) (l) -> tm (mtm)) (theta : (fin) (k) -> tm (mtm)) (Eq : forall x, ((funcomp) tau xi) x = theta x) : forall x, ((funcomp) (up_tm_tm tau) (upRen_tm_tm xi)) x = (up_tm_tm theta) x :=
+  fun n => match n with
+  | Some fin_n => (ap) (ren_tm (shift)) (Eq fin_n)
+  | None  => eq_refl
   end.
 
-Lemma upExt_tm_tm {m : nat} {n_tm : nat} (sigma : fin m -> tm n_tm)
-  (tau : fin m -> tm n_tm) (Eq : forall x, sigma x = tau x) :
-  forall x, up_tm_tm sigma x = up_tm_tm tau x.
-Proof.
-exact (fun n =>
-       match n with
-       | Some fin_n => ap (ren_tm shift) (Eq fin_n)
-       | None => eq_refl
-       end).
-Qed.
+Fixpoint compRenSubst_tm { ktm : nat } { ltm : nat } { mtm : nat } (xitm : (fin) (mtm) -> (fin) (ktm)) (tautm : (fin) (ktm) -> tm (ltm)) (thetatm : (fin) (mtm) -> tm (ltm)) (Eqtm : forall x, ((funcomp) tautm xitm) x = thetatm x) (s : tm (mtm)) : subst_tm tautm (ren_tm xitm s) = subst_tm thetatm s :=
+    match s return subst_tm tautm (ren_tm xitm s) = subst_tm thetatm s with
+    | var_tm (_) s => Eqtm s
+    | T (_)  => congr_T 
+    | F (_)  => congr_F 
+    | If (_) s0 s1 s2 => congr_If ((compRenSubst_tm xitm tautm thetatm Eqtm) s0) ((compRenSubst_tm xitm tautm thetatm Eqtm) s1) ((compRenSubst_tm xitm tautm thetatm Eqtm) s2)
+    | Lam (_) s0 s1 => congr_Lam ((fun x => (eq_refl) x) s0) ((compRenSubst_tm (upRen_tm_tm xitm) (up_tm_tm tautm) (up_tm_tm thetatm) (up_ren_subst_tm_tm (_) (_) (_) Eqtm)) s1)
+    | App (_) s0 s1 => congr_App ((compRenSubst_tm xitm tautm thetatm Eqtm) s0) ((compRenSubst_tm xitm tautm thetatm Eqtm) s1)
+    end.
 
-Lemma upExt_list_tm_tm {p : nat} {m : nat} {n_tm : nat}
-  (sigma : fin m -> tm n_tm) (tau : fin m -> tm n_tm)
-  (Eq : forall x, sigma x = tau x) :
-  forall x, up_list_tm_tm p sigma x = up_list_tm_tm p tau x.
-Proof.
-exact (fun n =>
-       scons_p_congr (fun n => eq_refl)
-         (fun n => ap (ren_tm (shift_p p)) (Eq n))).
-Qed.
-
-Fixpoint ext_tm {m_tm : nat} {n_tm : nat} (sigma_tm : fin m_tm -> tm n_tm)
-(tau_tm : fin m_tm -> tm n_tm) (Eq_tm : forall x, sigma_tm x = tau_tm x)
-(s : tm m_tm) {struct s} : subst_tm sigma_tm s = subst_tm tau_tm s :=
-  match s with
-  | var_tm _ s0 => Eq_tm s0
-  | Lam _ s0 s1 =>
-      congr_Lam (eq_refl s0)
-        (ext_tm (up_tm_tm sigma_tm) (up_tm_tm tau_tm) (upExt_tm_tm _ _ Eq_tm)
-           s1)
-  | App _ s0 s1 =>
-      congr_App (ext_tm sigma_tm tau_tm Eq_tm s0)
-        (ext_tm sigma_tm tau_tm Eq_tm s1)
+Definition up_subst_ren_tm_tm { k : nat } { ltm : nat } { mtm : nat } (sigma : (fin) (k) -> tm (ltm)) (zetatm : (fin) (ltm) -> (fin) (mtm)) (theta : (fin) (k) -> tm (mtm)) (Eq : forall x, ((funcomp) (ren_tm zetatm) sigma) x = theta x) : forall x, ((funcomp) (ren_tm (upRen_tm_tm zetatm)) (up_tm_tm sigma)) x = (up_tm_tm theta) x :=
+  fun n => match n with
+  | Some fin_n => (eq_trans) (compRenRen_tm (shift) (upRen_tm_tm zetatm) ((funcomp) (shift) zetatm) (fun x => eq_refl) (sigma fin_n)) ((eq_trans) ((eq_sym) (compRenRen_tm zetatm (shift) ((funcomp) (shift) zetatm) (fun x => eq_refl) (sigma fin_n))) ((ap) (ren_tm (shift)) (Eq fin_n)))
+  | None  => eq_refl
   end.
 
-Lemma up_ren_ren_tm_tm {k : nat} {l : nat} {m : nat} (xi : fin k -> fin l)
-  (zeta : fin l -> fin m) (rho : fin k -> fin m)
-  (Eq : forall x, funcomp zeta xi x = rho x) :
-  forall x, funcomp (upRen_tm_tm zeta) (upRen_tm_tm xi) x = upRen_tm_tm rho x.
-Proof.
-exact (up_ren_ren xi zeta rho Eq).
-Qed.
+Fixpoint compSubstRen_tm { ktm : nat } { ltm : nat } { mtm : nat } (sigmatm : (fin) (mtm) -> tm (ktm)) (zetatm : (fin) (ktm) -> (fin) (ltm)) (thetatm : (fin) (mtm) -> tm (ltm)) (Eqtm : forall x, ((funcomp) (ren_tm zetatm) sigmatm) x = thetatm x) (s : tm (mtm)) : ren_tm zetatm (subst_tm sigmatm s) = subst_tm thetatm s :=
+    match s return ren_tm zetatm (subst_tm sigmatm s) = subst_tm thetatm s with
+    | var_tm (_) s => Eqtm s
+    | T (_)  => congr_T 
+    | F (_)  => congr_F 
+    | If (_) s0 s1 s2 => congr_If ((compSubstRen_tm sigmatm zetatm thetatm Eqtm) s0) ((compSubstRen_tm sigmatm zetatm thetatm Eqtm) s1) ((compSubstRen_tm sigmatm zetatm thetatm Eqtm) s2)
+    | Lam (_) s0 s1 => congr_Lam ((fun x => (eq_refl) x) s0) ((compSubstRen_tm (up_tm_tm sigmatm) (upRen_tm_tm zetatm) (up_tm_tm thetatm) (up_subst_ren_tm_tm (_) (_) (_) Eqtm)) s1)
+    | App (_) s0 s1 => congr_App ((compSubstRen_tm sigmatm zetatm thetatm Eqtm) s0) ((compSubstRen_tm sigmatm zetatm thetatm Eqtm) s1)
+    end.
 
-Lemma up_ren_ren_list_tm_tm {p : nat} {k : nat} {l : nat} {m : nat}
-  (xi : fin k -> fin l) (zeta : fin l -> fin m) (rho : fin k -> fin m)
-  (Eq : forall x, funcomp zeta xi x = rho x) :
-  forall x,
-  funcomp (upRen_list_tm_tm p zeta) (upRen_list_tm_tm p xi) x =
-  upRen_list_tm_tm p rho x.
-Proof.
-exact (up_ren_ren_p Eq).
-Qed.
-
-Fixpoint compRenRen_tm {k_tm : nat} {l_tm : nat} {m_tm : nat}
-(xi_tm : fin m_tm -> fin k_tm) (zeta_tm : fin k_tm -> fin l_tm)
-(rho_tm : fin m_tm -> fin l_tm)
-(Eq_tm : forall x, funcomp zeta_tm xi_tm x = rho_tm x) (s : tm m_tm) {struct
- s} : ren_tm zeta_tm (ren_tm xi_tm s) = ren_tm rho_tm s :=
-  match s with
-  | var_tm _ s0 => ap (var_tm l_tm) (Eq_tm s0)
-  | Lam _ s0 s1 =>
-      congr_Lam (eq_refl s0)
-        (compRenRen_tm (upRen_tm_tm xi_tm) (upRen_tm_tm zeta_tm)
-           (upRen_tm_tm rho_tm) (up_ren_ren _ _ _ Eq_tm) s1)
-  | App _ s0 s1 =>
-      congr_App (compRenRen_tm xi_tm zeta_tm rho_tm Eq_tm s0)
-        (compRenRen_tm xi_tm zeta_tm rho_tm Eq_tm s1)
+Definition up_subst_subst_tm_tm { k : nat } { ltm : nat } { mtm : nat } (sigma : (fin) (k) -> tm (ltm)) (tautm : (fin) (ltm) -> tm (mtm)) (theta : (fin) (k) -> tm (mtm)) (Eq : forall x, ((funcomp) (subst_tm tautm) sigma) x = theta x) : forall x, ((funcomp) (subst_tm (up_tm_tm tautm)) (up_tm_tm sigma)) x = (up_tm_tm theta) x :=
+  fun n => match n with
+  | Some fin_n => (eq_trans) (compRenSubst_tm (shift) (up_tm_tm tautm) ((funcomp) (up_tm_tm tautm) (shift)) (fun x => eq_refl) (sigma fin_n)) ((eq_trans) ((eq_sym) (compSubstRen_tm tautm (shift) ((funcomp) (ren_tm (shift)) tautm) (fun x => eq_refl) (sigma fin_n))) ((ap) (ren_tm (shift)) (Eq fin_n)))
+  | None  => eq_refl
   end.
 
-Lemma up_ren_subst_tm_tm {k : nat} {l : nat} {m_tm : nat}
-  (xi : fin k -> fin l) (tau : fin l -> tm m_tm) (theta : fin k -> tm m_tm)
-  (Eq : forall x, funcomp tau xi x = theta x) :
-  forall x, funcomp (up_tm_tm tau) (upRen_tm_tm xi) x = up_tm_tm theta x.
-Proof.
-exact (fun n =>
-       match n with
-       | Some fin_n => ap (ren_tm shift) (Eq fin_n)
-       | None => eq_refl
-       end).
-Qed.
+Fixpoint compSubstSubst_tm { ktm : nat } { ltm : nat } { mtm : nat } (sigmatm : (fin) (mtm) -> tm (ktm)) (tautm : (fin) (ktm) -> tm (ltm)) (thetatm : (fin) (mtm) -> tm (ltm)) (Eqtm : forall x, ((funcomp) (subst_tm tautm) sigmatm) x = thetatm x) (s : tm (mtm)) : subst_tm tautm (subst_tm sigmatm s) = subst_tm thetatm s :=
+    match s return subst_tm tautm (subst_tm sigmatm s) = subst_tm thetatm s with
+    | var_tm (_) s => Eqtm s
+    | T (_)  => congr_T 
+    | F (_)  => congr_F 
+    | If (_) s0 s1 s2 => congr_If ((compSubstSubst_tm sigmatm tautm thetatm Eqtm) s0) ((compSubstSubst_tm sigmatm tautm thetatm Eqtm) s1) ((compSubstSubst_tm sigmatm tautm thetatm Eqtm) s2)
+    | Lam (_) s0 s1 => congr_Lam ((fun x => (eq_refl) x) s0) ((compSubstSubst_tm (up_tm_tm sigmatm) (up_tm_tm tautm) (up_tm_tm thetatm) (up_subst_subst_tm_tm (_) (_) (_) Eqtm)) s1)
+    | App (_) s0 s1 => congr_App ((compSubstSubst_tm sigmatm tautm thetatm Eqtm) s0) ((compSubstSubst_tm sigmatm tautm thetatm Eqtm) s1)
+    end.
 
-Lemma up_ren_subst_list_tm_tm {p : nat} {k : nat} {l : nat} {m_tm : nat}
-  (xi : fin k -> fin l) (tau : fin l -> tm m_tm) (theta : fin k -> tm m_tm)
-  (Eq : forall x, funcomp tau xi x = theta x) :
-  forall x,
-  funcomp (up_list_tm_tm p tau) (upRen_list_tm_tm p xi) x =
-  up_list_tm_tm p theta x.
-Proof.
-exact (fun n =>
-       eq_trans (scons_p_comp' _ _ _ n)
-         (scons_p_congr (fun z => scons_p_head' _ _ z)
-            (fun z =>
-             eq_trans (scons_p_tail' _ _ (xi z))
-               (ap (ren_tm (shift_p p)) (Eq z))))).
-Qed.
-
-Fixpoint compRenSubst_tm {k_tm : nat} {l_tm : nat} {m_tm : nat}
-(xi_tm : fin m_tm -> fin k_tm) (tau_tm : fin k_tm -> tm l_tm)
-(theta_tm : fin m_tm -> tm l_tm)
-(Eq_tm : forall x, funcomp tau_tm xi_tm x = theta_tm x) (s : tm m_tm) {struct
- s} : subst_tm tau_tm (ren_tm xi_tm s) = subst_tm theta_tm s :=
-  match s with
-  | var_tm _ s0 => Eq_tm s0
-  | Lam _ s0 s1 =>
-      congr_Lam (eq_refl s0)
-        (compRenSubst_tm (upRen_tm_tm xi_tm) (up_tm_tm tau_tm)
-           (up_tm_tm theta_tm) (up_ren_subst_tm_tm _ _ _ Eq_tm) s1)
-  | App _ s0 s1 =>
-      congr_App (compRenSubst_tm xi_tm tau_tm theta_tm Eq_tm s0)
-        (compRenSubst_tm xi_tm tau_tm theta_tm Eq_tm s1)
+Definition rinstInst_up_tm_tm { m : nat } { ntm : nat } (xi : (fin) (m) -> (fin) (ntm)) (sigma : (fin) (m) -> tm (ntm)) (Eq : forall x, ((funcomp) (var_tm (ntm)) xi) x = sigma x) : forall x, ((funcomp) (var_tm ((S) ntm)) (upRen_tm_tm xi)) x = (up_tm_tm sigma) x :=
+  fun n => match n with
+  | Some fin_n => (ap) (ren_tm (shift)) (Eq fin_n)
+  | None  => eq_refl
   end.
 
-Lemma up_subst_ren_tm_tm {k : nat} {l_tm : nat} {m_tm : nat}
-  (sigma : fin k -> tm l_tm) (zeta_tm : fin l_tm -> fin m_tm)
-  (theta : fin k -> tm m_tm)
-  (Eq : forall x, funcomp (ren_tm zeta_tm) sigma x = theta x) :
-  forall x,
-  funcomp (ren_tm (upRen_tm_tm zeta_tm)) (up_tm_tm sigma) x =
-  up_tm_tm theta x.
-Proof.
-exact (fun n =>
-       match n with
-       | Some fin_n =>
-           eq_trans
-             (compRenRen_tm shift (upRen_tm_tm zeta_tm)
-                (funcomp shift zeta_tm) (fun x => eq_refl) (sigma fin_n))
-             (eq_trans
-                (eq_sym
-                   (compRenRen_tm zeta_tm shift (funcomp shift zeta_tm)
-                      (fun x => eq_refl) (sigma fin_n)))
-                (ap (ren_tm shift) (Eq fin_n)))
-       | None => eq_refl
-       end).
-Qed.
+Fixpoint rinst_inst_tm { mtm : nat } { ntm : nat } (xitm : (fin) (mtm) -> (fin) (ntm)) (sigmatm : (fin) (mtm) -> tm (ntm)) (Eqtm : forall x, ((funcomp) (var_tm (ntm)) xitm) x = sigmatm x) (s : tm (mtm)) : ren_tm xitm s = subst_tm sigmatm s :=
+    match s return ren_tm xitm s = subst_tm sigmatm s with
+    | var_tm (_) s => Eqtm s
+    | T (_)  => congr_T 
+    | F (_)  => congr_F 
+    | If (_) s0 s1 s2 => congr_If ((rinst_inst_tm xitm sigmatm Eqtm) s0) ((rinst_inst_tm xitm sigmatm Eqtm) s1) ((rinst_inst_tm xitm sigmatm Eqtm) s2)
+    | Lam (_) s0 s1 => congr_Lam ((fun x => (eq_refl) x) s0) ((rinst_inst_tm (upRen_tm_tm xitm) (up_tm_tm sigmatm) (rinstInst_up_tm_tm (_) (_) Eqtm)) s1)
+    | App (_) s0 s1 => congr_App ((rinst_inst_tm xitm sigmatm Eqtm) s0) ((rinst_inst_tm xitm sigmatm Eqtm) s1)
+    end.
 
-Lemma up_subst_ren_list_tm_tm {p : nat} {k : nat} {l_tm : nat} {m_tm : nat}
-  (sigma : fin k -> tm l_tm) (zeta_tm : fin l_tm -> fin m_tm)
-  (theta : fin k -> tm m_tm)
-  (Eq : forall x, funcomp (ren_tm zeta_tm) sigma x = theta x) :
-  forall x,
-  funcomp (ren_tm (upRen_list_tm_tm p zeta_tm)) (up_list_tm_tm p sigma) x =
-  up_list_tm_tm p theta x.
-Proof.
-exact (fun n =>
-       eq_trans (scons_p_comp' _ _ _ n)
-         (scons_p_congr
-            (fun x => ap (var_tm (plus p m_tm)) (scons_p_head' _ _ x))
-            (fun n =>
-             eq_trans
-               (compRenRen_tm (shift_p p) (upRen_list_tm_tm p zeta_tm)
-                  (funcomp (shift_p p) zeta_tm)
-                  (fun x => scons_p_tail' _ _ x) (sigma n))
-               (eq_trans
-                  (eq_sym
-                     (compRenRen_tm zeta_tm (shift_p p)
-                        (funcomp (shift_p p) zeta_tm) (fun x => eq_refl)
-                        (sigma n))) (ap (ren_tm (shift_p p)) (Eq n)))))).
-Qed.
+Lemma rinstInst_tm { mtm : nat } { ntm : nat } (xitm : (fin) (mtm) -> (fin) (ntm)) : ren_tm xitm = subst_tm ((funcomp) (var_tm (ntm)) xitm) .
+Proof. exact ((FunctionalExtensionality.functional_extensionality _ _ ) (fun x => rinst_inst_tm xitm (_) (fun n => eq_refl) x)). Qed.
 
-Fixpoint compSubstRen_tm {k_tm : nat} {l_tm : nat} {m_tm : nat}
-(sigma_tm : fin m_tm -> tm k_tm) (zeta_tm : fin k_tm -> fin l_tm)
-(theta_tm : fin m_tm -> tm l_tm)
-(Eq_tm : forall x, funcomp (ren_tm zeta_tm) sigma_tm x = theta_tm x)
-(s : tm m_tm) {struct s} :
-ren_tm zeta_tm (subst_tm sigma_tm s) = subst_tm theta_tm s :=
-  match s with
-  | var_tm _ s0 => Eq_tm s0
-  | Lam _ s0 s1 =>
-      congr_Lam (eq_refl s0)
-        (compSubstRen_tm (up_tm_tm sigma_tm) (upRen_tm_tm zeta_tm)
-           (up_tm_tm theta_tm) (up_subst_ren_tm_tm _ _ _ Eq_tm) s1)
-  | App _ s0 s1 =>
-      congr_App (compSubstRen_tm sigma_tm zeta_tm theta_tm Eq_tm s0)
-        (compSubstRen_tm sigma_tm zeta_tm theta_tm Eq_tm s1)
-  end.
+Lemma instId_tm { mtm : nat } : subst_tm (var_tm (mtm)) = id .
+Proof. exact ((FunctionalExtensionality.functional_extensionality _ _ ) (fun x => idSubst_tm (var_tm (mtm)) (fun n => eq_refl) ((id) x))). Qed.
 
-Lemma up_subst_subst_tm_tm {k : nat} {l_tm : nat} {m_tm : nat}
-  (sigma : fin k -> tm l_tm) (tau_tm : fin l_tm -> tm m_tm)
-  (theta : fin k -> tm m_tm)
-  (Eq : forall x, funcomp (subst_tm tau_tm) sigma x = theta x) :
-  forall x,
-  funcomp (subst_tm (up_tm_tm tau_tm)) (up_tm_tm sigma) x = up_tm_tm theta x.
-Proof.
-exact (fun n =>
-       match n with
-       | Some fin_n =>
-           eq_trans
-             (compRenSubst_tm shift (up_tm_tm tau_tm)
-                (funcomp (up_tm_tm tau_tm) shift) (fun x => eq_refl)
-                (sigma fin_n))
-             (eq_trans
-                (eq_sym
-                   (compSubstRen_tm tau_tm shift
-                      (funcomp (ren_tm shift) tau_tm) (fun x => eq_refl)
-                      (sigma fin_n))) (ap (ren_tm shift) (Eq fin_n)))
-       | None => eq_refl
-       end).
-Qed.
+Lemma rinstId_tm { mtm : nat } : @ren_tm (mtm) (mtm) (id) = id .
+Proof. exact ((eq_trans) (rinstInst_tm ((id) (_))) instId_tm). Qed.
 
-Lemma up_subst_subst_list_tm_tm {p : nat} {k : nat} {l_tm : nat} {m_tm : nat}
-  (sigma : fin k -> tm l_tm) (tau_tm : fin l_tm -> tm m_tm)
-  (theta : fin k -> tm m_tm)
-  (Eq : forall x, funcomp (subst_tm tau_tm) sigma x = theta x) :
-  forall x,
-  funcomp (subst_tm (up_list_tm_tm p tau_tm)) (up_list_tm_tm p sigma) x =
-  up_list_tm_tm p theta x.
-Proof.
-exact (fun n =>
-       eq_trans
-         (scons_p_comp' (funcomp (var_tm (plus p l_tm)) (zero_p p)) _ _ n)
-         (scons_p_congr
-            (fun x => scons_p_head' _ (fun z => ren_tm (shift_p p) _) x)
-            (fun n =>
-             eq_trans
-               (compRenSubst_tm (shift_p p) (up_list_tm_tm p tau_tm)
-                  (funcomp (up_list_tm_tm p tau_tm) (shift_p p))
-                  (fun x => eq_refl) (sigma n))
-               (eq_trans
-                  (eq_sym
-                     (compSubstRen_tm tau_tm (shift_p p) _
-                        (fun x => eq_sym (scons_p_tail' _ _ x)) (sigma n)))
-                  (ap (ren_tm (shift_p p)) (Eq n)))))).
-Qed.
+Lemma varL_tm { mtm : nat } { ntm : nat } (sigmatm : (fin) (mtm) -> tm (ntm)) : (funcomp) (subst_tm sigmatm) (var_tm (mtm)) = sigmatm .
+Proof. exact ((FunctionalExtensionality.functional_extensionality _ _ ) (fun x => eq_refl)). Qed.
 
-Fixpoint compSubstSubst_tm {k_tm : nat} {l_tm : nat} {m_tm : nat}
-(sigma_tm : fin m_tm -> tm k_tm) (tau_tm : fin k_tm -> tm l_tm)
-(theta_tm : fin m_tm -> tm l_tm)
-(Eq_tm : forall x, funcomp (subst_tm tau_tm) sigma_tm x = theta_tm x)
-(s : tm m_tm) {struct s} :
-subst_tm tau_tm (subst_tm sigma_tm s) = subst_tm theta_tm s :=
-  match s with
-  | var_tm _ s0 => Eq_tm s0
-  | Lam _ s0 s1 =>
-      congr_Lam (eq_refl s0)
-        (compSubstSubst_tm (up_tm_tm sigma_tm) (up_tm_tm tau_tm)
-           (up_tm_tm theta_tm) (up_subst_subst_tm_tm _ _ _ Eq_tm) s1)
-  | App _ s0 s1 =>
-      congr_App (compSubstSubst_tm sigma_tm tau_tm theta_tm Eq_tm s0)
-        (compSubstSubst_tm sigma_tm tau_tm theta_tm Eq_tm s1)
-  end.
+Lemma varLRen_tm { mtm : nat } { ntm : nat } (xitm : (fin) (mtm) -> (fin) (ntm)) : (funcomp) (ren_tm xitm) (var_tm (mtm)) = (funcomp) (var_tm (ntm)) xitm .
+Proof. exact ((FunctionalExtensionality.functional_extensionality _ _ ) (fun x => eq_refl)). Qed.
 
-Lemma renRen_tm {k_tm : nat} {l_tm : nat} {m_tm : nat}
-  (xi_tm : fin m_tm -> fin k_tm) (zeta_tm : fin k_tm -> fin l_tm)
-  (s : tm m_tm) :
-  ren_tm zeta_tm (ren_tm xi_tm s) = ren_tm (funcomp zeta_tm xi_tm) s.
-Proof.
-exact (compRenRen_tm xi_tm zeta_tm _ (fun n => eq_refl) s).
-Qed.
+Lemma compComp_tm { ktm : nat } { ltm : nat } { mtm : nat } (sigmatm : (fin) (mtm) -> tm (ktm)) (tautm : (fin) (ktm) -> tm (ltm)) (s : tm (mtm)) : subst_tm tautm (subst_tm sigmatm s) = subst_tm ((funcomp) (subst_tm tautm) sigmatm) s .
+Proof. exact (compSubstSubst_tm sigmatm tautm (_) (fun n => eq_refl) s). Qed.
 
-Lemma renRen'_tm_pointwise {k_tm : nat} {l_tm : nat} {m_tm : nat}
-  (xi_tm : fin m_tm -> fin k_tm) (zeta_tm : fin k_tm -> fin l_tm) :
-  pointwise_relation _ eq (funcomp (ren_tm zeta_tm) (ren_tm xi_tm))
-    (ren_tm (funcomp zeta_tm xi_tm)).
-Proof.
-exact (fun s => compRenRen_tm xi_tm zeta_tm _ (fun n => eq_refl) s).
-Qed.
+Lemma compComp'_tm { ktm : nat } { ltm : nat } { mtm : nat } (sigmatm : (fin) (mtm) -> tm (ktm)) (tautm : (fin) (ktm) -> tm (ltm)) : (funcomp) (subst_tm tautm) (subst_tm sigmatm) = subst_tm ((funcomp) (subst_tm tautm) sigmatm) .
+Proof. exact ((FunctionalExtensionality.functional_extensionality _ _ ) (fun n => compComp_tm sigmatm tautm n)). Qed.
 
-Lemma renSubst_tm {k_tm : nat} {l_tm : nat} {m_tm : nat}
-  (xi_tm : fin m_tm -> fin k_tm) (tau_tm : fin k_tm -> tm l_tm) (s : tm m_tm)
-  : subst_tm tau_tm (ren_tm xi_tm s) = subst_tm (funcomp tau_tm xi_tm) s.
-Proof.
-exact (compRenSubst_tm xi_tm tau_tm _ (fun n => eq_refl) s).
-Qed.
+Lemma compRen_tm { ktm : nat } { ltm : nat } { mtm : nat } (sigmatm : (fin) (mtm) -> tm (ktm)) (zetatm : (fin) (ktm) -> (fin) (ltm)) (s : tm (mtm)) : ren_tm zetatm (subst_tm sigmatm s) = subst_tm ((funcomp) (ren_tm zetatm) sigmatm) s .
+Proof. exact (compSubstRen_tm sigmatm zetatm (_) (fun n => eq_refl) s). Qed.
 
-Lemma renSubst_tm_pointwise {k_tm : nat} {l_tm : nat} {m_tm : nat}
-  (xi_tm : fin m_tm -> fin k_tm) (tau_tm : fin k_tm -> tm l_tm) :
-  pointwise_relation _ eq (funcomp (subst_tm tau_tm) (ren_tm xi_tm))
-    (subst_tm (funcomp tau_tm xi_tm)).
-Proof.
-exact (fun s => compRenSubst_tm xi_tm tau_tm _ (fun n => eq_refl) s).
-Qed.
+Lemma compRen'_tm { ktm : nat } { ltm : nat } { mtm : nat } (sigmatm : (fin) (mtm) -> tm (ktm)) (zetatm : (fin) (ktm) -> (fin) (ltm)) : (funcomp) (ren_tm zetatm) (subst_tm sigmatm) = subst_tm ((funcomp) (ren_tm zetatm) sigmatm) .
+Proof. exact ((FunctionalExtensionality.functional_extensionality _ _ ) (fun n => compRen_tm sigmatm zetatm n)). Qed.
 
-Lemma substRen_tm {k_tm : nat} {l_tm : nat} {m_tm : nat}
-  (sigma_tm : fin m_tm -> tm k_tm) (zeta_tm : fin k_tm -> fin l_tm)
-  (s : tm m_tm) :
-  ren_tm zeta_tm (subst_tm sigma_tm s) =
-  subst_tm (funcomp (ren_tm zeta_tm) sigma_tm) s.
-Proof.
-exact (compSubstRen_tm sigma_tm zeta_tm _ (fun n => eq_refl) s).
-Qed.
+Lemma renComp_tm { ktm : nat } { ltm : nat } { mtm : nat } (xitm : (fin) (mtm) -> (fin) (ktm)) (tautm : (fin) (ktm) -> tm (ltm)) (s : tm (mtm)) : subst_tm tautm (ren_tm xitm s) = subst_tm ((funcomp) tautm xitm) s .
+Proof. exact (compRenSubst_tm xitm tautm (_) (fun n => eq_refl) s). Qed.
 
-Lemma substRen_tm_pointwise {k_tm : nat} {l_tm : nat} {m_tm : nat}
-  (sigma_tm : fin m_tm -> tm k_tm) (zeta_tm : fin k_tm -> fin l_tm) :
-  pointwise_relation _ eq (funcomp (ren_tm zeta_tm) (subst_tm sigma_tm))
-    (subst_tm (funcomp (ren_tm zeta_tm) sigma_tm)).
-Proof.
-exact (fun s => compSubstRen_tm sigma_tm zeta_tm _ (fun n => eq_refl) s).
-Qed.
+Lemma renComp'_tm { ktm : nat } { ltm : nat } { mtm : nat } (xitm : (fin) (mtm) -> (fin) (ktm)) (tautm : (fin) (ktm) -> tm (ltm)) : (funcomp) (subst_tm tautm) (ren_tm xitm) = subst_tm ((funcomp) tautm xitm) .
+Proof. exact ((FunctionalExtensionality.functional_extensionality _ _ ) (fun n => renComp_tm xitm tautm n)). Qed.
 
-Lemma substSubst_tm {k_tm : nat} {l_tm : nat} {m_tm : nat}
-  (sigma_tm : fin m_tm -> tm k_tm) (tau_tm : fin k_tm -> tm l_tm)
-  (s : tm m_tm) :
-  subst_tm tau_tm (subst_tm sigma_tm s) =
-  subst_tm (funcomp (subst_tm tau_tm) sigma_tm) s.
-Proof.
-exact (compSubstSubst_tm sigma_tm tau_tm _ (fun n => eq_refl) s).
-Qed.
+Lemma renRen_tm { ktm : nat } { ltm : nat } { mtm : nat } (xitm : (fin) (mtm) -> (fin) (ktm)) (zetatm : (fin) (ktm) -> (fin) (ltm)) (s : tm (mtm)) : ren_tm zetatm (ren_tm xitm s) = ren_tm ((funcomp) zetatm xitm) s .
+Proof. exact (compRenRen_tm xitm zetatm (_) (fun n => eq_refl) s). Qed.
 
-Lemma substSubst_tm_pointwise {k_tm : nat} {l_tm : nat} {m_tm : nat}
-  (sigma_tm : fin m_tm -> tm k_tm) (tau_tm : fin k_tm -> tm l_tm) :
-  pointwise_relation _ eq (funcomp (subst_tm tau_tm) (subst_tm sigma_tm))
-    (subst_tm (funcomp (subst_tm tau_tm) sigma_tm)).
-Proof.
-exact (fun s => compSubstSubst_tm sigma_tm tau_tm _ (fun n => eq_refl) s).
-Qed.
+Lemma renRen'_tm { ktm : nat } { ltm : nat } { mtm : nat } (xitm : (fin) (mtm) -> (fin) (ktm)) (zetatm : (fin) (ktm) -> (fin) (ltm)) : (funcomp) (ren_tm zetatm) (ren_tm xitm) = ren_tm ((funcomp) zetatm xitm) .
+Proof. exact ((FunctionalExtensionality.functional_extensionality _ _ ) (fun n => renRen_tm xitm zetatm n)). Qed.
 
-Lemma rinstInst_up_tm_tm {m : nat} {n_tm : nat} (xi : fin m -> fin n_tm)
-  (sigma : fin m -> tm n_tm)
-  (Eq : forall x, funcomp (var_tm n_tm) xi x = sigma x) :
-  forall x, funcomp (var_tm (S n_tm)) (upRen_tm_tm xi) x = up_tm_tm sigma x.
-Proof.
-exact (fun n =>
-       match n with
-       | Some fin_n => ap (ren_tm shift) (Eq fin_n)
-       | None => eq_refl
-       end).
-Qed.
+End tm.
 
-Lemma rinstInst_up_list_tm_tm {p : nat} {m : nat} {n_tm : nat}
-  (xi : fin m -> fin n_tm) (sigma : fin m -> tm n_tm)
-  (Eq : forall x, funcomp (var_tm n_tm) xi x = sigma x) :
-  forall x,
-  funcomp (var_tm (plus p n_tm)) (upRen_list_tm_tm p xi) x =
-  up_list_tm_tm p sigma x.
-Proof.
-exact (fun n =>
-       eq_trans (scons_p_comp' _ _ (var_tm (plus p n_tm)) n)
-         (scons_p_congr (fun z => eq_refl)
-            (fun n => ap (ren_tm (shift_p p)) (Eq n)))).
-Qed.
+Arguments var_tm {ntm}.
 
-Fixpoint rinst_inst_tm {m_tm : nat} {n_tm : nat}
-(xi_tm : fin m_tm -> fin n_tm) (sigma_tm : fin m_tm -> tm n_tm)
-(Eq_tm : forall x, funcomp (var_tm n_tm) xi_tm x = sigma_tm x) (s : tm m_tm)
-{struct s} : ren_tm xi_tm s = subst_tm sigma_tm s :=
-  match s with
-  | var_tm _ s0 => Eq_tm s0
-  | Lam _ s0 s1 =>
-      congr_Lam (eq_refl s0)
-        (rinst_inst_tm (upRen_tm_tm xi_tm) (up_tm_tm sigma_tm)
-           (rinstInst_up_tm_tm _ _ Eq_tm) s1)
-  | App _ s0 s1 =>
-      congr_App (rinst_inst_tm xi_tm sigma_tm Eq_tm s0)
-        (rinst_inst_tm xi_tm sigma_tm Eq_tm s1)
-  end.
+Arguments T {ntm}.
 
-Lemma rinstInst'_tm {m_tm : nat} {n_tm : nat} (xi_tm : fin m_tm -> fin n_tm)
-  (s : tm m_tm) : ren_tm xi_tm s = subst_tm (funcomp (var_tm n_tm) xi_tm) s.
-Proof.
-exact (rinst_inst_tm xi_tm _ (fun n => eq_refl) s).
-Qed.
+Arguments F {ntm}.
 
-Lemma rinstInst'_tm_pointwise {m_tm : nat} {n_tm : nat}
-  (xi_tm : fin m_tm -> fin n_tm) :
-  pointwise_relation _ eq (ren_tm xi_tm)
-    (subst_tm (funcomp (var_tm n_tm) xi_tm)).
-Proof.
-exact (fun s => rinst_inst_tm xi_tm _ (fun n => eq_refl) s).
-Qed.
+Arguments If {ntm}.
 
-Lemma instId'_tm {m_tm : nat} (s : tm m_tm) : subst_tm (var_tm m_tm) s = s.
-Proof.
-exact (idSubst_tm (var_tm m_tm) (fun n => eq_refl) s).
-Qed.
+Arguments Lam {ntm}.
 
-Lemma instId'_tm_pointwise {m_tm : nat} :
-  pointwise_relation _ eq (subst_tm (var_tm m_tm)) id.
-Proof.
-exact (fun s => idSubst_tm (var_tm m_tm) (fun n => eq_refl) s).
-Qed.
+Arguments App {ntm}.
 
-Lemma rinstId'_tm {m_tm : nat} (s : tm m_tm) : ren_tm id s = s.
-Proof.
-exact (eq_ind_r (fun t => t = s) (instId'_tm s) (rinstInst'_tm id s)).
-Qed.
+Global Instance Subst_tm { mtm : nat } { ntm : nat } : Subst1 ((fin) (mtm) -> tm (ntm)) (tm (mtm)) (tm (ntm)) := @subst_tm (mtm) (ntm) .
 
-Lemma rinstId'_tm_pointwise {m_tm : nat} :
-  pointwise_relation _ eq (@ren_tm m_tm m_tm id) id.
-Proof.
-exact (fun s => eq_ind_r (fun t => t = s) (instId'_tm s) (rinstInst'_tm id s)).
-Qed.
+Global Instance Ren_tm { mtm : nat } { ntm : nat } : Ren1 ((fin) (mtm) -> (fin) (ntm)) (tm (mtm)) (tm (ntm)) := @ren_tm (mtm) (ntm) .
 
-Lemma varL'_tm {m_tm : nat} {n_tm : nat} (sigma_tm : fin m_tm -> tm n_tm)
-  (x : fin m_tm) : subst_tm sigma_tm (var_tm m_tm x) = sigma_tm x.
-Proof.
-exact (eq_refl).
-Qed.
+Global Instance VarInstance_tm { mtm : nat } : Var ((fin) (mtm)) (tm (mtm)) := @var_tm (mtm) .
 
-Lemma varL'_tm_pointwise {m_tm : nat} {n_tm : nat}
-  (sigma_tm : fin m_tm -> tm n_tm) :
-  pointwise_relation _ eq (funcomp (subst_tm sigma_tm) (var_tm m_tm))
-    sigma_tm.
-Proof.
-exact (fun x => eq_refl).
-Qed.
+Notation "x '__tm'" := (var_tm x) (at level 5, format "x __tm") : subst_scope.
 
-Lemma varLRen'_tm {m_tm : nat} {n_tm : nat} (xi_tm : fin m_tm -> fin n_tm)
-  (x : fin m_tm) : ren_tm xi_tm (var_tm m_tm x) = var_tm n_tm (xi_tm x).
-Proof.
-exact (eq_refl).
-Qed.
+Notation "x '__tm'" := (@ids (_) (_) VarInstance_tm x) (at level 5, only printing, format "x __tm") : subst_scope.
 
-Lemma varLRen'_tm_pointwise {m_tm : nat} {n_tm : nat}
-  (xi_tm : fin m_tm -> fin n_tm) :
-  pointwise_relation _ eq (funcomp (ren_tm xi_tm) (var_tm m_tm))
-    (funcomp (var_tm n_tm) xi_tm).
-Proof.
-exact (fun x => eq_refl).
-Qed.
+Notation "'var'" := (var_tm) (only printing, at level 1) : subst_scope.
 
-Class Up_tm X Y :=
-    up_tm : X -> Y.
+Class Up_tm X Y := up_tm : X -> Y.
 
-#[global]
-Instance Subst_tm  {m_tm n_tm : nat}: (Subst1 _ _ _) := (@subst_tm m_tm n_tm).
+Notation "↑__tm" := (up_tm) (only printing) : subst_scope.
 
-#[global]
-Instance Up_tm_tm  {m n_tm : nat}: (Up_tm _ _) := (@up_tm_tm m n_tm).
+Notation "↑__tm" := (up_tm_tm) (only printing) : subst_scope.
 
-#[global]
-Instance Ren_tm  {m_tm n_tm : nat}: (Ren1 _ _ _) := (@ren_tm m_tm n_tm).
+Global Instance Up_tm_tm { m : nat } { ntm : nat } : Up_tm (_) (_) := @up_tm_tm (m) (ntm) .
 
-#[global]
-Instance VarInstance_tm  {n_tm : nat}: (Var _ _) := (@var_tm n_tm).
+Notation "s [ sigmatm ]" := (subst_tm sigmatm s) (at level 7, left associativity, only printing) : subst_scope.
 
-Notation "[ sigma_tm ]" := (subst_tm sigma_tm)
-( at level 1, left associativity, only printing)  : fscope.
+Notation "[ sigmatm ]" := (subst_tm sigmatm) (at level 1, left associativity, only printing) : fscope.
 
-Notation "s [ sigma_tm ]" := (subst_tm sigma_tm s)
-( at level 7, left associativity, only printing)  : subst_scope.
+Notation "s ⟨ xitm ⟩" := (ren_tm xitm s) (at level 7, left associativity, only printing) : subst_scope.
 
-Notation "↑__tm" := up_tm (only printing)  : subst_scope.
+Notation "⟨ xitm ⟩" := (ren_tm xitm) (at level 1, left associativity, only printing) : fscope.
 
-Notation "↑__tm" := up_tm_tm (only printing)  : subst_scope.
+Ltac auto_unfold := repeat unfold subst1,  subst2,  Subst1,  Subst2,  ids,  ren1,  ren2,  Ren1,  Ren2,  Subst_tm,  Ren_tm,  VarInstance_tm.
 
-Notation "⟨ xi_tm ⟩" := (ren_tm xi_tm)
-( at level 1, left associativity, only printing)  : fscope.
+Tactic Notation "auto_unfold" "in" "*" := repeat unfold subst1,  subst2,  Subst1,  Subst2,  ids,  ren1,  ren2,  Ren1,  Ren2,  Subst_tm,  Ren_tm,  VarInstance_tm in *.
 
-Notation "s ⟨ xi_tm ⟩" := (ren_tm xi_tm s)
-( at level 7, left associativity, only printing)  : subst_scope.
+Ltac asimpl' := repeat first [progress rewrite ?instId_tm| progress rewrite ?compComp_tm| progress rewrite ?compComp'_tm| progress rewrite ?rinstId_tm| progress rewrite ?compRen_tm| progress rewrite ?compRen'_tm| progress rewrite ?renComp_tm| progress rewrite ?renComp'_tm| progress rewrite ?renRen_tm| progress rewrite ?renRen'_tm| progress rewrite ?varL_tm| progress rewrite ?varLRen_tm| progress (unfold up_ren, upRen_tm_tm, up_tm_tm)| progress (cbn [subst_tm ren_tm])| fsimpl].
 
-Notation "'var'" := var_tm ( at level 1, only printing)  : subst_scope.
-
-Notation "x '__tm'" := (@ids _ _ VarInstance_tm x)
-( at level 5, format "x __tm", only printing)  : subst_scope.
-
-Notation "x '__tm'" := (var_tm x) ( at level 5, format "x __tm")  :
-subst_scope.
-
-#[global]
-Instance subst_tm_morphism  {m_tm : nat} {n_tm : nat}:
- (Proper (respectful (pointwise_relation _ eq) (respectful eq eq))
-    (@subst_tm m_tm n_tm)).
-Proof.
-exact (fun f_tm g_tm Eq_tm s t Eq_st =>
-       eq_ind s (fun t' => subst_tm f_tm s = subst_tm g_tm t')
-         (ext_tm f_tm g_tm Eq_tm s) t Eq_st).
-Qed.
-
-#[global]
-Instance subst_tm_morphism2  {m_tm : nat} {n_tm : nat}:
- (Proper (respectful (pointwise_relation _ eq) (pointwise_relation _ eq))
-    (@subst_tm m_tm n_tm)).
-Proof.
-exact (fun f_tm g_tm Eq_tm s => ext_tm f_tm g_tm Eq_tm s).
-Qed.
-
-#[global]
-Instance ren_tm_morphism  {m_tm : nat} {n_tm : nat}:
- (Proper (respectful (pointwise_relation _ eq) (respectful eq eq))
-    (@ren_tm m_tm n_tm)).
-Proof.
-exact (fun f_tm g_tm Eq_tm s t Eq_st =>
-       eq_ind s (fun t' => ren_tm f_tm s = ren_tm g_tm t')
-         (extRen_tm f_tm g_tm Eq_tm s) t Eq_st).
-Qed.
-
-#[global]
-Instance ren_tm_morphism2  {m_tm : nat} {n_tm : nat}:
- (Proper (respectful (pointwise_relation _ eq) (pointwise_relation _ eq))
-    (@ren_tm m_tm n_tm)).
-Proof.
-exact (fun f_tm g_tm Eq_tm s => extRen_tm f_tm g_tm Eq_tm s).
-Qed.
-
-Ltac auto_unfold := repeat
-                     unfold VarInstance_tm, Var, ids, Ren_tm, Ren1, ren1,
-                      Up_tm_tm, Up_tm, up_tm, Subst_tm, Subst1, subst1.
-
-Tactic Notation "auto_unfold" "in" "*" := repeat
-                                           unfold VarInstance_tm, Var, ids,
-                                            Ren_tm, Ren1, ren1, Up_tm_tm,
-                                            Up_tm, up_tm, Subst_tm, Subst1,
-                                            subst1 in *.
-
-Ltac asimpl' := repeat (first
-                 [ progress setoid_rewrite substSubst_tm_pointwise
-                 | progress setoid_rewrite substSubst_tm
-                 | progress setoid_rewrite substRen_tm_pointwise
-                 | progress setoid_rewrite substRen_tm
-                 | progress setoid_rewrite renSubst_tm_pointwise
-                 | progress setoid_rewrite renSubst_tm
-                 | progress setoid_rewrite renRen'_tm_pointwise
-                 | progress setoid_rewrite renRen_tm
-                 | progress setoid_rewrite varLRen'_tm_pointwise
-                 | progress setoid_rewrite varLRen'_tm
-                 | progress setoid_rewrite varL'_tm_pointwise
-                 | progress setoid_rewrite varL'_tm
-                 | progress setoid_rewrite rinstId'_tm_pointwise
-                 | progress setoid_rewrite rinstId'_tm
-                 | progress setoid_rewrite instId'_tm_pointwise
-                 | progress setoid_rewrite instId'_tm
-                 | progress
-                    unfold up_list_tm_tm, up_tm_tm, upRen_list_tm_tm,
-                     upRen_tm_tm, up_ren
-                 | progress cbn[subst_tm ren_tm]
-                 | progress fsimpl ]).
-
-Ltac asimpl := check_no_evars;
-                repeat
-                 unfold VarInstance_tm, Var, ids, Ren_tm, Ren1, ren1,
-                  Up_tm_tm, Up_tm, up_tm, Subst_tm, Subst1, subst1 in *;
-                asimpl'; minimize.
+Ltac asimpl := repeat try unfold_funcomp; auto_unfold in *; asimpl'; repeat try unfold_funcomp.
 
 Tactic Notation "asimpl" "in" hyp(J) := revert J; asimpl; intros J.
 
-Tactic Notation "auto_case" := auto_case ltac:(asimpl; cbn; eauto).
+Tactic Notation "auto_case" := auto_case (asimpl; cbn; eauto).
 
-Ltac substify := auto_unfold; try setoid_rewrite rinstInst'_tm_pointwise;
-                  try setoid_rewrite rinstInst'_tm.
+Tactic Notation "asimpl" "in" "*" := auto_unfold in *; repeat first [progress rewrite ?instId_tm in *| progress rewrite ?compComp_tm in *| progress rewrite ?compComp'_tm in *| progress rewrite ?rinstId_tm in *| progress rewrite ?compRen_tm in *| progress rewrite ?compRen'_tm in *| progress rewrite ?renComp_tm in *| progress rewrite ?renComp'_tm in *| progress rewrite ?renRen_tm in *| progress rewrite ?renRen'_tm in *| progress rewrite ?varL_tm in *| progress rewrite ?varLRen_tm in *| progress (unfold up_ren, upRen_tm_tm, up_tm_tm in *)| progress (cbn [subst_tm ren_tm] in *)| fsimpl in *].
 
-Ltac renamify := auto_unfold; try setoid_rewrite_left rinstInst'_tm_pointwise;
-                  try setoid_rewrite_left rinstInst'_tm.
+Ltac substify := auto_unfold; try repeat (erewrite rinstInst_tm).
 
-End Core.
-
-Module Extra.
-
-Import
-Core.
-
-Arguments var_tm {n_tm}.
-
-Arguments App {n_tm}.
-
-Arguments Lam {n_tm}.
-
-#[global]Hint Opaque subst_tm: rewrite.
-
-#[global]Hint Opaque ren_tm: rewrite.
-
-End Extra.
-
-Module interface.
-
-Export Core.
-
-Export Extra.
-
-End interface.
-
-Export interface.
-
+Ltac renamify := auto_unfold; try repeat (erewrite <- rinstInst_tm).
