stlc_norm/norm.v
@@ -1,0 +1,206 @@
+Require Export stlc.
+Require Import ssreflect.
+
+(* Set Implicit Arguments. *)
+(* Unset Strict Implicit. *)
+(* Unset Printing Implicit Defensive. *)
+
+Definition context n := fin n -> ty.
+
+Definition empty_ctx : context 0 :=
+  fun x => match x with end.
+
+Inductive value {n} : tm n -> Prop :=
+  | VTrue : value T
+  | VFalse : value F
+  | VLam : forall typ t, value (Lam typ t).
+
+Inductive has_ty {n} (ctx : context n) : tm n -> ty -> Prop :=
+  | TVar : forall x, has_ty ctx (var_tm x) (ctx x)
+  | TLam : forall t x T1 T2,
+      has_ty (T1 .: ctx) t T2 -> has_ty ctx (Lam x t) (Fun T1 T2)
+  | TApp : forall t1 t2 T1 T2,
+      has_ty ctx t2 T1 -> has_ty ctx t1 (Fun T1 T2) -> has_ty ctx (App t1 t2) T2
+  | TTrue : has_ty ctx T Bool
+  | TFalse : has_ty ctx F Bool
+  | TIf : forall t1 t2 t3 typ,
+      has_ty ctx t1 Bool ->
+      has_ty ctx t2 typ ->
+      has_ty ctx t3 typ ->
+      has_ty ctx (If t1 t2 t3) typ.
+
+Hint Constructors has_ty : core.
+
+Inductive big_step {n} : tm n -> tm n -> Prop :=
+  | FunDone : forall type t, big_step (Lam type t) (Lam type t)
+  | TDone : big_step T T
+  | FDone : big_step F F
+  | ST_App : forall e1 e2 e v v' type,
+      big_step e1 (Lam type e) ->
+      big_step e2 v ->
+      big_step (subst_tm (v..) e) v' ->
+      big_step (App e1 e2) v'
+  | ST_IfT : forall e1 e2 e3 v,
+      big_step e1 T ->
+      big_step e2 v ->
+      big_step (If e1 e2 e3) v
+  | ST_IfF : forall e1 e2 e3 v,
+      big_step e1 F ->
+      big_step e3 v ->
+      big_step (If e1 e2 e3) v.
+
+Hint Constructors big_step : core.
+
+Example test : big_step (App (Lam Bool ((@var_tm 1) var_zero)) T) T.
+Proof. eauto. Qed.
+
+Definition norm {n} (t : tm n) := exists t', big_step t t'.
+
+Fixpoint N (type : ty) (t : tm 0) : Prop :=
+  has_ty empty_ctx t type /\ norm t /\
+  match type with
+  | Bool => True
+  | Fun t1 t2 => forall t', N t1 t' -> N t2 (App t t')
+  end.
+
+Lemma N_impl_norm : forall t type, N type t -> norm t.
+Proof.
+  move=> t type. elim: type => [_ _ _ _|] [_ [? _]] //.
+Qed.
+
+Lemma N_impl_type : forall t typ, N typ t -> has_ty empty_ctx t typ.
+Proof.
+  move=> t typ. by elim: typ => [? _ ? _|] [H _].
+Qed.
+
+Definition sub n m := fin n -> tm m.
+Definition sub_ok_in {n} (sub : sub n 0) (ctx : context n) :=
+  forall i, N (ctx i) (sub i).
+
+Definition good_ren {n m} (ren : fin n -> fin m) (ctx : context n) ctx' :=
+  forall i, ctx i = ctx' (ren i).
+Definition good_sub {n m} (sub : sub n m) ctx ctx' :=
+  forall i, has_ty ctx' (sub i) (ctx i).
+
+Lemma good_ren_cons {n m} (ren : fin n -> fin m) ctx ctx' typ :
+  good_ren ren ctx ctx' ->
+  good_ren (up_ren ren) (typ .: ctx) (typ .: ctx').
+Proof.
+  rewrite /good_ren. move=> ?. by case.
+Qed.
+
+Lemma renaming {n} : forall e typ ctx m ctx' (ren : fin n -> fin m),
+  has_ty ctx e typ ->
+  good_ren ren ctx ctx' ->
+  has_ty ctx' (ren_tm ren e) typ.
+Proof.
+  move=> e typ ctx + + + Hty. induction Hty; try (intros; asimpl; eauto).
+  - rewrite /good_ren in H. by rewrite H.
+  - asimpl. econstructor. eauto using good_ren_cons.
+Qed.
+
+Lemma weakening {n} : forall (t : tm n) typ typ' ctx,
+  has_ty ctx t typ ->
+  has_ty (typ' .: ctx) (ren_tm shift t) typ.
+Proof.
+  intros. eapply renaming; eauto. by unfold good_ren.
+Qed.
+
+Lemma good_sub_cons {n m} (sub : sub n m) ctx ctx' typ :
+  good_sub sub ctx ctx' ->
+  good_sub (up_tm sub) (typ .: ctx) (typ .: ctx').
+Proof.
+  unfold good_sub. intros. destruct i.
+  - by apply weakening.
+  - constructor.
+Qed.
+
+Lemma sub_ok_impl_good {n} : forall (s : sub n 0) ctx,
+  sub_ok_in s ctx -> good_sub s ctx empty_ctx.
+Proof.
+  rewrite /sub_ok_in/good_sub. auto using N_impl_type.
+Qed.
+
+Lemma sub_ok_cons {n} : forall (s : sub n 0) ctx (t : tm 0) typ,
+  sub_ok_in s ctx ->
+  N typ t ->
+  sub_ok_in (t .: s) (typ .: ctx).
+Proof.
+  rewrite /sub_ok_in. move=>> ? ? i. by case: i.
+Qed.
+
+Lemma morphing : forall n e m ctx ctx' (sub : sub n m) typ,
+  has_ty ctx e typ ->
+  good_sub sub ctx ctx' ->
+  has_ty ctx' (subst_tm sub e) typ.
+Proof.
+  induction e; simpl; move=>> H; inversion H; eauto using good_sub_cons.
+Qed.
+
+Lemma preservation {n} : forall (t t' : tm n) typ ctx,
+  big_step t t' ->
+  has_ty ctx t typ ->
+  has_ty ctx t' typ.
+Proof.
+  move=> t t' + + Hstep. induction Hstep => typ ctx Hty; inversion Hty; auto.
+  apply IHHstep3. apply IHHstep1 in H3. inversion H3; subst.
+  eapply morphing.
+  + eassumption.
+  + rewrite /good_sub. induction i; [constructor|auto].
+Qed.
+
+Lemma big_step_to_val {n} : forall (t v : tm n), big_step t v -> value v.
+Proof.
+  Hint Constructors value : core.
+  induction 1; auto.
+Qed.
+
+Lemma N_backpreservation : forall typ t v,
+  big_step t v ->
+  N typ v ->
+  N typ t.
+Admitted.
+
+Lemma N_preservation : forall typ t v,
+  big_step t v ->
+  N typ t ->
+  N typ v.
+Admitted.
+
+Lemma canonical_forms_bool : forall v,
+  value v ->
+  has_ty empty_ctx v Bool ->
+  (v = T \/ v = F).
+Proof.
+  intros. inversion H; auto.
+  - subst. inversion H0.
+Qed.
+
+Lemma fundamental_lemma : forall ctx (t : tm 0) typ sub,
+  has_ty ctx t typ ->
+  sub_ok_in sub ctx ->
+  N typ (subst_tm sub t).
+Proof.
+  move=> ctx t typ sub Hty.
+  induction Hty.
+  - done.
+  - move=> Hsub. repeat split.
+    + eauto using morphing, sub_ok_impl_good.
+    + exists (subst_tm sub (Lam x t)). by simpl.
+    + move=> t' /[dup] /N_impl_norm Hnorm HN. destruct Hnorm as [v Hv].
+      assert (sub_ok_in (v .: sub) (T1 .: ctx)); eauto using sub_ok_cons, N_preservation.
+      * apply IHHty in H. move: H => /[dup] /N_impl_norm Hnormt HNt. destruct Hnormt as [v' Hv'].
+        -- simpl. apply N_backpreservation with (v := v').
+           ++ econstructor; eauto. asimpl => //.
+           ++ eapply N_preservation; eauto.
+  - simpl. intros. apply IHHty2; [|apply IHHty1]; assumption.
+  - by repeat split; try exists T.
+  - by repeat split; try exists F.
+  - move=> /[dup] Hsub Hsub'. simpl. apply IHHty1 in Hsub. destruct Hsub as [Hty [[v Hv] _]].
+    move: Hv => /[dup] Hv Hv2. apply big_step_to_val in Hv. apply canonical_forms_bool in Hv.
+    + case: Hv => Hv; subst; [apply IHHty2 in Hsub'|apply IHHty3 in Hsub'];
+      move: Hsub' => /[dup] /N_impl_norm Hnorm HN; destruct Hnorm as [v' Hv'];
+        eapply N_backpreservation; eauto;
+        eapply N_preservation; eauto.
+    + by apply (preservation (subst_tm sub t1)).
+Qed.
